Bump Rust + RefinedRust versions (#112)
* bump RefinedRust + Rust
* update readme

---------

Signed-off-by: Lennard Gäher <l.gaeher@posteo.de>

security-monitor/rust-crates/pointers_utility/src/lib.rs
@@ -3,13 +3,13 @@
 // SPDX-License-Identifier: Apache-2.0
 #![no_std]
 #![no_main]
-#![feature(pointer_byte_offsets)]
 
 // used for RefinedRust annotations
 #![feature(register_tool)]
 #![register_tool(rr)]
 #![feature(custom_inner_attributes)]
 #![rr::coq_prefix("ace_ptr")]
+#![rr::include("stdlib")]
 
 
 mod error;
@@ -17,8 +17,11 @@ use core::mem::size_of;
 pub use crate::error::PointerError;
 
 /// Calculates the offset in bytes between two pointers. 
+#[rr::only_spec]
+#[rr::returns("wrap_to_it (pointer1.2 - pointer2.2) isize")]
 pub fn ptr_byte_offset(pointer1: *const usize, pointer2: *const usize) -> isize {
-    (pointer1 as isize) - (pointer2 as isize)
+    // TODO: we should use wrapping arithmetic here, as it might overflow
+    (pointer1.addr() as isize) - (pointer2.addr() as isize)
 }
 
 /// Aligns the pointer to specific size while making sure that the aligned pointer
@@ -34,11 +37,9 @@ pub fn ptr_align(pointer: *mut usize, align_in_bytes: usize, owned_region_end: *
 /// the one-past-the-end address. The returned pointer is guaranteed to be valid for accesses
 /// of size one, if the original pointer is valid. Additional checks are required for making
 /// larger memory accesses.
-#[rr::skip]
-#[rr::params("l", "off", "lmax")]
-#[rr::args("l", "off", "lmax")]
-#[rr::requires("⌜l.2 + off < lmax.2⌝")]
-#[rr::returns("Ok(l +ₗ off)")]
+#[rr::ok]
+#[rr::requires("pointer.2 + offset_in_bytes < owned_region_end.2")]
+#[rr::ensures("ret = (pointer +ₗ offset_in_bytes)")]
 pub fn ptr_byte_add_mut(
     pointer: *mut usize, offset_in_bytes: usize, owned_region_end: *const usize,
 ) -> Result<*mut usize, PointerError> {
@@ -59,6 +60,9 @@ pub fn ptr_byte_add_mut(
 /// the one-past-the-end address. The returned pointer is guaranteed to be valid for accesses
 /// of size one, if the original pointer is valid. Additional checks are required for making
 /// larger memory accesses.
+#[rr::ok]
+#[rr::requires("pointer.2 + offset_in_bytes < owned_region_end.2")]
+#[rr::ensures("ret = (pointer +ₗ offset_in_bytes)")]
 pub fn ptr_byte_add(
     pointer: *const usize, offset_in_bytes: usize, owned_region_end: *const usize,
 ) -> Result<*const usize, PointerError> {
