security-monitor/src/core/panic.rs
@@ -13,7 +13,7 @@ fn panic(info: &core::panic::PanicInfo) -> ! {
     // TODO: halt all other harts and make sure the below code executes exclusively on one hart
     debug!("Ops security monitor panicked!");
     match info.location() {
-        Some(p) => debug!("Line {}, file {}: {}", p.line(), p.file(), info.message().unwrap()),
+        Some(p) => debug!("Line {}, file {}: {}", p.line(), p.file(), info.message()),
         None => debug!("no information available."),
     }
     debug!("Cleaning up...");
