security-monitor/src/lib.rs
@@ -4,16 +4,7 @@
 #![no_std]
 #![no_main]
 #![feature(
-    // used for meaningful panic code
-    panic_info_message,
-    // used for calculating offsets for assembly
-    asm_const,
-    // const_mut_ref for LinkedList implementation used in the heap allocator
-    const_mut_refs,
-    pointer_is_aligned,
-    // pointer_is_aligned_to,
-    result_option_inspect,
-    pointer_byte_offsets,
+    pointer_is_aligned_to,
     // used for formal verification framework (RefinedRust annotations)
     register_tool,
     custom_inner_attributes,
@@ -22,11 +13,8 @@
 // RefinedRust configuration
 #![register_tool(rr)]
 #![rr::coq_prefix("sm")]
-#![rr::include("spin")]
-#![rr::include("alloc")]
-#![rr::include("vec")]
-#![rr::include("option")]
-#![rr::include("result")]
+#![rr::include("stdlib")]
+#![rr::include("pointers_utility")]
 
 extern crate alloc;
 
