verification/rust_proofs/ace/proofs/proof_core_page_allocator_page_Page_core_page_allocator_page_UnAllocated_divide_closure0.v
@@ -1,0 +1,48 @@
+From caesium Require Import lang notation.
+From refinedrust Require Import typing shims.
+From sm.ace.generated Require Import generated_code_ace generated_specs_ace generated_template_core_page_allocator_page_Page_core_page_allocator_page_UnAllocated_divide_closure0.
+
+Set Default Proof Using "Type".
+
+Section proof.
+Context `{RRGS : !refinedrustGS Σ}.
+
+Lemma core_page_allocator_page_Page_core_page_allocator_page_UnAllocated_divide_closure0_proof (π : thread_id) :
+  core_page_allocator_page_Page_core_page_allocator_page_UnAllocated_divide_closure0_lemma π.
+Proof.
+  core_page_allocator_page_Page_core_page_allocator_page_UnAllocated_divide_closure0_prelude.
+
+  rep <-! liRStep; liShow.
+  apply_update (updateable_copy_lft "vlft7" "ulft5").
+  rep <-! liRStep; liShow.
+  apply_update (updateable_copy_lft "plft21" "vlft7").
+  rep <-! liRStep; liShow.
+  apply_update (updateable_copy_lft "vlft9" "ulft5").
+  rep <-! liRStep; liShow.
+  apply_update (updateable_copy_lft "vlft11" "ulft5").
+  rep <-! liRStep; liShow.
+  apply_update (updateable_copy_lft "plft24" "vlft11").
+  rep <-! liRStep; liShow.
+  apply_update (updateable_copy_lft "plft22" "ulft5").
+  rep <-! liRStep; liShow.
+  rename select (if_Err _ _) into Herr.
+  rename select (if_Ok _ _) into Hok.
+  destruct x' as [ | x']; first last.
+  { exfalso. simpl in *. apply Herr. split; last lia.
+    move: Hinrange Hpage_end. unfold page_size_in_bytes_Z. lia. }
+  simpl in *. revert Hok.
+  rep liRStep.
+
+  all: print_remaining_goal.
+  Unshelve. all: sidecond_solver.
+  Unshelve. all: sidecond_hammer.
+  - (* add *)
+    eapply aligned_to_offset.
+    { apply Haligned. }
+    rewrite page_size_align_is_size /page_size_in_bytes_Z.
+    apply Z.divide_factor_r.
+  - move: Hinrange Hpage_end. rewrite /page_size_in_bytes_Z. nia.
+
+  Unshelve. all: print_remaining_sidecond.
+Admitted. (* admitted due to admit_proofs config flag *)
+End proof.
