verification/rust_proofs/ace/proofs/proof_core_page_allocator_page_Page_core_page_allocator_page_UnAllocated_init.v
@@ -18,5 +18,5 @@ Proof.
   Unshelve. all: sidecond_solver.
   Unshelve. all: sidecond_hammer.
   Unshelve. all: print_remaining_sidecond.
-Admitted. (* admitted due to admit_proofs config flag *)
+Qed.
 End proof.
